Util/Vector/VecOrd.v
@@ -253,12 +253,12 @@ Arguments Vrel1_app_impl [A R n v1 v2] _.
 Arguments Vrel1_sub [A R n v1 v2 p q] h _.
 
 (***********************************************************************)
-(** Compatibility of [Vrel1] with [same_relation]. *)
+(** Compatibility of [Vrel1] with [same_rel]. *)
 
 Require Import Morphisms.
 
 Instance Vrel1_app_same_rel n A :
-  Proper (same_relation ==> same_relation) (@Vrel1_app n A).
+  Proper (same_rel ==> same_rel) (@Vrel1_app n A).
 
 Proof.
   intros R R' RR'. rewrite rel_eq. intros v1 v2. unfold Vrel1.
@@ -266,8 +266,7 @@ Proof.
     ex i vi x j vj h y; fo.
 Qed.
 
-Instance Vrel1_same_rel n A :
-  Proper (same_relation ==> same_relation) (@Vrel1 n A).
+Instance Vrel1_same_rel n A : Proper (same_rel ==> same_rel) (@Vrel1 n A).
 
 Proof.
   intros R R' RR'. rewrite 2!Vrel1_app_eq. apply Vrel1_app_same_rel. hyp.
